<?xml version="1.0" encoding="UTF-8"?>
<exercises>
  <exercise>
    <statement>
      <p>
        What is the difference between a Taylor polynomial and a Taylor series?
        </p>
    </statement>
    <answer>
      <p>
        A Taylor polynomial is a <em>polynomial</em>, containing a finite number of terms. A Taylor series is a <em>series</em>, the summation of an infinite number of terms.
      </p>
    </answer>
  </exercise>
  <exercise>
    <statement>
      <p>
        What theorem must we use to show that a function is equal to its Taylor series?
        </p>
    </statement>
    <answer>
      <p>
        <xref ref="thm_function_series_equality" />
      </p>
    </answer>
  </exercise>
  <exercisegroup>
    <introduction>
      <p>
        <xref ref="idea_common_taylor" /> gives the <m>n^\text{th}</m> term of the Taylor series of common functions. In Exercises 3–6, verify the formula given in the Key Idea by finding the first few terms of the Taylor series of the given function and identifying a pattern.
      </p>
    </introduction>
    <exercise>
      <statement>
        <p>
          <m>f(x) = e^x</m>; <m>c=0</m>
        </p>
      </statement>
      <answer>
        <p>
          All derivatives of <m>e^x</m> are <m>e^x</m> which evaluate to 1 at <m>x=0</m>.
        </p>
        <p>
          The Taylor series starts <m>1+x+\frac{1}{2}x^2+\frac{1}{3!}x^3+\frac{1}{4!}x^4+\cdots </m>;
        </p>
        <p>
          the Taylor series is <m>\displaystyle \sum _{n=0}^\infty \frac{x^n}{n!}</m>
        </p>
      </answer>
    </exercise>
    <exercise>
      <statement>
        <p>
          <m>f(x) = \sin x</m>; <m>c=0</m>
        </p>
      </statement>
      <answer>
        <p>
          All derivatives of <m>\sin x</m> are either <m>\pm \cos x</m> or <m>\pm \sin x</m>, which evaluate to <m>\pm 1</m> or <m>0</m> at <m>x=0</m>. The Taylor series starts <m>0+x+0x^2-\frac{1}{6}x^3+0x^4+\frac{1}{120}x^5</m>;
        </p>
        <p>
          the Taylor series is <m>\displaystyle \sum _{n=0}^\infty (-1)^n\frac{x^{2n+1}}{(2n+1)!}</m>
        </p>
      </answer>
    </exercise>
    <exercise>
      <statement>
        <p>
          <m>f(x) = 1/(1-x)</m>; <m>c=0</m>
        </p>
      </statement>
      <answer>
        <p>
          The <m>n^\text{th}</m> derivative of <m>1/(1-x)</m> is <m>f\,^{(n)}(x) = (n)!/(1-x)^{n+1}</m>, which evaluates to <m>n!</m> at <m>x=0</m>.
        </p>
        <p>
          The Taylor series starts <m>1+x+x^2+x^3+\cdots </m>;
        </p>
        <p>
          the Taylor series is <m>\displaystyle \sum _{n=0}^\infty x^n</m>
        </p>
      </answer>
    </exercise>
    <exercise>
      <statement>
        <p>
          <m>f(x) = \tan ^{-1}x</m>; <m>c=0</m>
        </p>
      </statement>
      <answer>
        <p>
          The derivative of <m>\tan ^{-1}x</m> is <m>1/(1+x^2)</m>. Taking successive derivatives using the Quotient Rule, the derivatives of <m>\tan ^{-1}x</m> fall into two categories in terms of their evaluation at <m>x=0</m>.
        </p>
        <p>
          When <m>n</m> is even, <m>\displaystyle f\,^{(n)}(x) = (-1)^{(n-1)/2}\frac{p(x)}{(1+x^2)^n}</m>, where <m>p(x)</m> is a polynomial such that <m>p(0) = 0</m>. Hence <m>f\,^{(n)}(0) = 0</m> when <m>n</m> is even.
        </p>
        <p>
          When <m>n</m> is odd, <m>\displaystyle f\,^{(n)}(x) = (-1)^{(n-1)/2}\frac{p(x)}{(1+x^2)^n}</m>, where <m>p(x)</m> is a polynomial such that <m>p(0) = (n-1)!</m>. Hence <m>f\,^{(n)}(0) = (-1)^{(n-1)/2}(n-1)!</m> when <m>n</m> is odd. (The unusual power of <m>(-1)</m> is such that every other odd term is negative.)
        </p>
        <p>
          The Taylor series starts <m>x-\frac{1}{3}x^3+\frac{1}{5}x^5+\cdots </m>; by reindexing to only obtain odd powers of <m>x</m>, we get
        </p>
        <p>
          the Taylor series is <m>\displaystyle \sum _{n=0}^\infty (-1)^n\frac{x^{2n+1}}{2n+1}</m>.
        </p>
      </answer>
    </exercise>
  </exercisegroup>
  <exercisegroup>
    <introduction>
      <p>
        In Exercises 7–12, find a formula for the <m>n^\text{th}</m> term of the Taylor series of <m>f(x)</m>, centered at <m>c</m>, by finding the coefficients of the first few powers of <m>x</m> and looking for a pattern. (The formulas for several of these are found in <xref ref="idea_common_taylor" />; show work verifying these formula.)
      </p>
    </introduction>
    <exercise>
      <statement>
        <p>
          <m>f(x) = \cos x</m>; <m>c=\pi /2</m>
        </p>
      </statement>
      <answer>
        <p>
          The Taylor series starts <m>0-(x-\pi /2)+0x^2+\frac{1}{6}(x-\pi /2)^3+0x^4-\frac{1}{120}(x-\pi /2)^5</m>;
        </p>
        <p>
          the Taylor series is <m>\displaystyle \sum _{n=0}^\infty (-1)^{n+1}\frac{(x-\pi /2)^{2n+1}}{(2n+1)!}</m>
        </p>
      </answer>
    </exercise>
    <exercise>
      <statement>
        <p>
          <m>f(x) = 1/x</m>; <m>c=1</m>
        </p>
      </statement>
      <answer>
        <p>
          The Taylor series starts <m>1-(x-1)+(x-1)^2-(x-1)^3+(x-1)^4-(x-1)^5</m>;
        </p>
        <p>
          the Taylor series is <m>\displaystyle \sum _{n=0}^\infty (-1)^{n}(x-1)^n</m>
        </p>
      </answer>
    </exercise>
    <exercise>
      <statement>
        <p>
          <m>f(x) = e^{-x}</m>; <m>c=0</m>
        </p>
      </statement>
      <answer>
        <p>
          <m>f\,^{(n)}(x) = (-1)^ne^{-x}</m>; at <m>x=0</m>, <m>f\,^{(n)}(0)=-1</m> when <m>n</m> is odd and <m>f\,^{(n)}(0)=1</m> when <m>n</m> is even.</p>
        <p>
          The Taylor series starts <m>1-x+\frac{1}{2}x^2-\frac{1}{3!}x^3+\cdots </m>;
        </p>
        <p>
          the Taylor series is <m>\displaystyle \sum _{n=0}^\infty (-1)^n\frac{x^n}{n!}</m>.
        </p>
      </answer>
    </exercise>
    <exercise>
      <statement>
        <p>
          <m>f(x) = \ln (1+x)</m>; <m>c=0</m>
        </p>
      </statement>
      <answer>
        <p>
          <m>f\,^{(n)}(x) = (-1)^{n+1}\frac{(n-1)!}{(1+x)^n}</m>; at <m>x=0</m>, <m>f\,^{(n)}(0)=(-1)^{n+1}(n-1)!</m>
        </p>
        <p>
          The Taylor series starts <m>x-\frac{x^2}{2}+\frac{x^3}{3}-\frac{x^4}{4}+\cdots </m>;
        </p>
        <p>
          the Taylor series is <m>\displaystyle \sum _{n=1}^\infty (-1)^{n+1}\frac{x^n}{n}</m>.
        </p>
      </answer>
    </exercise>
    <exercise>
      <statement>
        <p>
          <m>f(x) = x/(x+1)</m>; <m>c=1</m>
        </p>
      </statement>
      <answer>
        <p>
          <m>f\,^{(n)}(x) = (-1)^{n+1}\frac{n!}{(x+1)^{n+1}}</m>; at <m>x=1</m>, <m>f\,^{(n)}(1)=(-1)^{n+1}\frac{n!}{2^{n+1}}</m>
        </p>
        <p>
          The Taylor series starts <m>\frac{1}{2}+\frac{1}{4}(x-1)-\frac{1}{8}(x-1)^2+\frac{1}{16}(x-1)^3\cdots </m>;
        </p>
        <p>
          the Taylor series is <m>\displaystyle \frac{1}{2}+\sum _{n=1}^\infty (-1)^{n+1}\frac{(x-1)^n}{2^{n+1}}</m>.
        </p>
      </answer>
    </exercise>
    <exercise>
      <statement>
        <p>
          <m>f(x) = \sin x</m>; <m>c=\pi /4</m>
        </p>
      </statement>
      <answer>
        <p>
          The derivatives of <m>\sin x</m> are <m>\pm \cos x</m> and <m>\pm \sin x</m>; at <m>x=\pi /4</m>, these derivatives evaluate to <m>\pm \sqrt{2}/2</m>.
        </p>
        <p>
          The Taylor series starts <m>\frac{\sqrt{2}}{2}+\frac{\sqrt{2}}{2}(x-\pi /4) - \frac{\sqrt{2}}{2}\frac{(x-\pi /4)^2}{2}-\frac{\sqrt{2}}{2}\frac{(x-\pi /4)^3}{3!}+\frac{\sqrt{2}}{2}\frac{(x-\pi /4)^4}{4!}+\frac{\sqrt{2}}{2}\frac{(x-\pi /4)^5}{5!}\cdots </m>. Note how the signs are “even, even, odd, odd, even, even, odd, odd,<m>\ldots </m>” We saw signs like these in <xref ref="ex_seq2" />; one way of producing such signs is to raise <m>(-1)</m> to a special quadratic power. While many possibilities exist, one such quadratic is <m>(n+3)(n+4)/2</m>.
        </p>
        <p>
          Thus the Taylor series is <m>\displaystyle \sum _{n=0}^\infty (-1)^{\frac{(n+3)(n+4)}{2}}\frac{\sqrt{2}}{2}\frac{(x-\pi /4)^n}{n!}</m>.
        </p>
      </answer>
    </exercise>
  </exercisegroup>
  <exercisegroup>
    <introduction>
      <p>
        In Exercises 13–16, show that the Taylor series for <m>f(x)</m>, as given in <xref ref="idea_common_taylor" />, is equal to <m>f(x)</m> by applying <xref ref="thm_taylorthm" />; that is, show <m>\displaystyle \lim _{n\rightarrow \infty }R_n(x) =0</m>.
      </p>
    </introduction>
    <exercise>
      <statement>
        <p>
          <m>f(x) = e^x</m>
        </p>
      </statement>
      <answer>
        <p>
          Given a value <m>x</m>, the magnitude of the error term <m>R_n(x)</m> is bounded by<md>
            <mrow> \big |R_n(x)\big | \le \frac{\max \left|\,f\,^{(n+1)}(z)\right|}{(n+1)!}\big |x^{(n+1)}\big |,</mrow>
          </md>
          where <m>z</m> is between <m>0</m> and <m>x</m>.
        </p>
        <p>
          If <m>x\gt0</m>, then <m>z\lt x</m> and <m>f\,^{(n+1)}(z) =e^z\lt e^x</m>. If <m>x\lt 0</m>, then <m>x\lt z\lt 0</m> and <m>f\,^{(n+1)}(z) =e^z\lt 1</m>. So given a fixed <m>x</m> value, let <m>M = \max \lbrace e^x,1\rbrace </m>; <m>f\,^{(n)}(z)\lt M.</m> This allows us to state<md>
            <mrow> \big |R_n(x)\big | \le \frac{M}{(n+1)!}\big |x^{(n+1)}\big |.</mrow>
          </md>
          For any <m>x</m>, <m>\displaystyle \lim _{n\rightarrow \infty } \frac{M}{(n+1)!}\big |x^{(n+1)}\big |= 0</m>. Thus by the Squeeze Theorem, we conclude that <m>\displaystyle \lim _{n\rightarrow \infty } R_n(x) = 0</m> for all <m>x</m>, and hence<md>
            <mrow>e^x = \sum _{n=0}^\infty \frac{x^{n}}{n!}\quad \text{for all $x$}.</mrow>
          </md>
          
        </p>
      </answer>
    </exercise>
    <exercise>
      <statement>
        <p>
          <m>f(x) = \sin x</m>
        </p>
      </statement>
      <answer>
        <p>
          The following argument is essentially the same as that given for <m>f(x) = \cos x</m> in <xref ref="ex_ts1" />.
        </p>
        <p>
          Given a value <m>x</m>, the magnitude of the error term <m>R_n(x)</m> is bounded by<md>
            <mrow> \big |R_n(x)\big | \le \frac{\max \left|\,f\,^{(n+1)}(z)\right|}{(n+1)!}\big |x^{(n+1)}\big |.</mrow>
          </md>
          Since all derivatives of <m>\sin x</m> are <m>\pm \cos x</m> or <m>\pm \sin x</m>, whose magnitudes are bounded by <m>1</m>, we can state<md>
            <mrow> \big |R_n(x)\big | \le \frac{1}{(n+1)!}\big |x^{(n+1)}\big |.</mrow>
          </md>
          For any <m>x</m>, <m>\displaystyle \lim _{n\rightarrow \infty } \frac{x^{n+1}}{(n+1)!} = 0</m>. Thus by the Squeeze Theorem, we conclude that <m>\displaystyle \lim _{n\rightarrow \infty } R_n(x) = 0</m> for all <m>x</m>, and hence<md>
            <mrow>\sin x = \sum _{n=0}^\infty (-1)^{n}\frac{x^{2n+1}}{(2n+1)!}\quad \text{for all $x$}.</mrow>
          </md>
          
        </p>
      </answer>
    </exercise>
    <exercise>
      <statement>
        <p>
          <m>f(x) = \ln x</m> (show equality only on <m>(1,2)</m>)</p>
      </statement>
      <answer>
        <p>
          Given a value <m>x</m>, the magnitude of the error term <m>R_n(x)</m> is bounded by<md>
            <mrow> \big |R_n(x)\big | \le \frac{\max \left|\,f\,^{(n+1)}(z)\right|}{(n+1)!}\big |(x-1)^{(n+1)}\big |,</mrow>
          </md>
          where <m>z</m> is between <m>1</m> and <m>x</m>.
        </p>
        <p>
          Note that <m>\big |f\,^{(n+1)}(x)\big | = \frac{n!}{x^{n+1}}</m>.
        </p>
        <p>
          Per the statement of the problem, we only consider the case <m>1\lt x\lt 2</m>.
        </p>
        <p>
          If <m>1\lt x\lt 2</m>, then <m>1\lt z\lt x</m> and <m>f\,^{(n+1)}(z) =\frac{n!}{z^{n+1}}\lt n!</m>. Thus<md>
            <mrow> \big |R_n(x)\big | \le \frac{n!}{(n+1)!}\big |(x-1)^{(n+1)}\big |= \frac{(x-1)^{n+1}}{n+1}\lt \frac{1}{n+1}.</mrow>
          </md>
          Thus<md>
            <mrow>\lim _{n\rightarrow \infty } \big |R_n(x)\big | \lt  \lim _{n\rightarrow \infty } \frac{1}{n+1}=0,</mrow>
          </md>
          hence<md>
            <mrow>\ln x = \sum _{n=1}^\infty (-1)^{n+1}\frac{(x-1)^n}{n}\ \text{on}\ (1,2).</mrow>
          </md>
          
        </p>
      </answer>
    </exercise>
    <exercise>
      <statement>
        <p>
          <m>f(x) = 1/(1-x)</m> (show equality only on <m>(-1,0)</m>)</p>
      </statement>
      <answer>
        <p>
          Given a value <m>x</m>, the magnitude of the error term <m>R_n(x)</m> is bounded by<md>
            <mrow> \big |R_n(x)\big | \le \frac{\max \left|\,f\,^{(n+1)}(z)\right|}{(n+1)!}\big |x^{(n+1)}\big |,</mrow>
          </md>
          where <m>z</m> is between <m>0</m> and <m>x</m>.
        </p>
        <p>
          Note that <m>\big |f\,^{(n+1)}(x)\big | = \frac{(n+1)!}{(1-x)^{n+2}}</m>.
        </p>
        <p>
          If <m>-1\lt x\lt 0</m>, then <m>x\lt z\lt 0</m> and <m>f\,^{(n+1)}(z) =\frac{(n+1)!}{(1-z)^{n+2}}\lt (n+1)!</m>. Thus<md>
            <mrow> \big |R_n(x)\big | \le \frac{(n+1)!}{(n+1)!}\big |x^{n+1}\big |= \big |x^{n+1}\big |.</mrow>
          </md>
          For a fixed <m>x</m>,<md>
            <mrow>\lim _{n\rightarrow \infty } \big |x^{n+1}\big |=0 \text{ as } |x|\lt 1,</mrow>
          </md>
          hence<md>
            <mrow>\frac{1}{1-x} = \sum _{n=0}^\infty x^n \text{ on } (-1,0).</mrow>
          </md>
          
        </p>
      </answer>
    </exercise>
  </exercisegroup>
  <exercisegroup>
    <introduction>
      <p>
        In Exercises 17–20, use the Taylor series given in <xref ref="idea_common_taylor" /> to verify the given identity.
      </p>
    </introduction>
    <exercise>
      <statement>
        <p>
          <m>\cos (-x) = \cos x</m>
        </p>
      </statement>
      <answer>
        <p>
          Given <m>\displaystyle \cos x = \sum _{n=0}^\infty (-1)^n\frac{x^{2n}}{(2n)!}</m>,
        </p>
        <p>
          <m>\displaystyle \cos (-x) = \sum _{n=0}^\infty (-1)^n\frac{(-x)^{2n}}{(2n)!}=\sum _{n=0}^\infty (-1)^n\frac{x^{2n}}{(2n)!}=\cos x</m>, as all powers in the series are even.</p>
      </answer>
    </exercise>
    <exercise>
      <statement>
        <p>
          <m>\sin (-x) = -\sin x</m>
        </p>
      </statement>
      <answer>
        <p>
          Given <m>\displaystyle \sin x = \sum _{n=0}^\infty (-1)^n\frac{x^{2n+1}}{(2n+1)!}</m>,
        </p>
        <p>
          <m>\displaystyle \sin (-x) = \sum _{n=0}^\infty (-1)^n\frac{(-x)^{2n+1}}{(2n+1)!}=\sum _{n=0}^\infty (-1)^n\frac{-x^{2n+1}}{(2n+1)!}=-\sin x</m>, as all powers in the series are odd.</p>
      </answer>
    </exercise>
    <exercise>
      <statement>
        <p>
          <m>\frac{d}{dx}\big (\sin x\big ) = \cos x</m>
        </p>
      </statement>
      <answer>
        <p>
          Given <m>\displaystyle \sin x = \sum _{n=0}^\infty (-1)^n\frac{x^{2n+1}}{(2n+1)!}</m>,
        </p>
        <p>
          <m>\displaystyle \frac{d}{dx}\big (\sin x\big ) = \frac{d}{dx}\left(\sum _{n=0}^\infty (-1)^n\frac{x^{2n+1}}{(2n+1)!}\right)=\sum _{n=0}^\infty (-1)^n\frac{(2n+1)x^{2n}}{(2n+1)!}=\sum _{n=0}^\infty (-1)^n\frac{x^{2n}}{(2n)!}=\cos x</m>. (The summation still starts at <m>n=0</m> as there was no constant term in the expansion of <m>\sin x</m>).</p>
      </answer>
    </exercise>
    <exercise>
      <statement>
        <p>
          <m>\frac{d}{dx}\big (\cos x\big ) = -\sin x</m>
        </p>
      </statement>
      <answer>
        <p>
          Given <m>\displaystyle \cos x = \sum _{n=0}^\infty (-1)^n\frac{x^{2n}}{(2n)!}</m>,
        </p>
        <p>
          <m>\displaystyle \frac{d}{dx}\big (\cos x\big ) = \frac{d}{dx}\left(\sum _{n=0}^\infty (-1)^n\frac{x^{2n}}{(2n)!}\right)=\sum _{n=1}^\infty (-1)^n\frac{(2n)x^{2n-1}}{(2n)!}=\sum _{n=1}^\infty (-1)^n\frac{x^{2n-1}}{(2n-1)!}</m>. We can re-index this summation to start at <m>n=0</m> by replacing <m>n</m> with <m>n+1</m> in the summation:<md>
            <mrow> \sum _{n=1}^\infty (-1)^n\frac{x^{2n-1}}{(2n-1)!} =\sum _{n=0}^\infty (-1)^{n+1}\frac{x^{2n+1}}{(2n+1)!}.</mrow>
          </md>
        </p>
        <p>
          Note that this series has the opposite sign of the Taylor series for <m>\sin x</m>; thus <m>\frac{d}{dx}(\cos x) = -\sin x</m>.
        </p>
      </answer>
    </exercise>
  </exercisegroup>
  <exercisegroup>
    <introduction>
      <p>
        In Exercises 21–24, write out the first 5 terms of the Binomial series with the given <m>k</m>-value.
      </p>
    </introduction>
    <exercise>
      <statement>
        <p>
          <m>k=1/2</m>
        </p>
      </statement>
      <answer>
        <p>
          <m>\displaystyle 1+\frac{x}{2}-\frac{x^2}{8}+\frac{x^3}{16}-\frac{5x^4}{128}</m>
        </p>
      </answer>
    </exercise>
    <exercise>
      <statement>
        <p>
          <m>k=-1/2</m>
        </p>
      </statement>
      <answer>
        <p>
          <m>\displaystyle 1-\frac{x}{2}+\frac{3x^2}{8}-\frac{5x^3}{16}+\frac{35x^4}{128}</m>
        </p>
      </answer>
    </exercise>
    <exercise>
      <statement>
        <p>
          <m>k=1/3</m>
        </p>
      </statement>
      <answer>
        <p>
          <m>\displaystyle 1+\frac{x}{3}-\frac{x^2}{9}+\frac{5x^3}{81}-\frac{10x^4}{243}</m>
        </p>
      </answer>
    </exercise>
    <exercise>
      <statement>
        <p>
          <m>k=4</m>
        </p>
      </statement>
      <answer>
        <p>
          <m>\displaystyle 1+4x+6x^2+4x^3+x^4</m> (note the series is finite, and the formula still applies)</p>
      </answer>
    </exercise>
  </exercisegroup>
  <exercisegroup>
    <introduction>
      <p>
        In Exercises 25–30, use the Taylor series given in <xref ref="idea_common_taylor" /> to create the Taylor series of the given functions.
      </p>
    </introduction>
    <exercise>
      <statement>
        <p>
          <m>f(x) = \cos \big (x^2\big )</m>
        </p>
      </statement>
      <answer>
        <p>
          <m>\displaystyle \sum _{n=0}^\infty (-1)^n\frac{(x^2)^{2n}}{(2n)!} = \sum _{n=0}^\infty (-1)^n\frac{x^{4n}}{(2n)!}.</m>
        </p>
      </answer>
    </exercise>
    <exercise>
      <statement>
        <p>
          <m>f(x) = e^{-x}</m>
        </p>
      </statement>
      <answer>
        <p>
          <m>\displaystyle \sum _{n=0}^\infty \frac{(-x)^n}{n!}.</m>
        </p>
      </answer>
    </exercise>
    <exercise>
      <statement>
        <p>
          <m>f(x) = \sin \big (2x+3\big )</m>
        </p>
      </statement>
      <answer>
        <p>
          <m>\displaystyle \sum _{n=0}^\infty (-1)^n\frac{(2x+3)^{2n+1}}{(2n+1)!}.</m>
        </p>
      </answer>
    </exercise>
    <exercise>
      <statement>
        <p>
          <m>f(x) = \tan ^{-1}\big (x/2\big )</m>
        </p>
      </statement>
      <answer>
        <p>
          <m>\displaystyle \sum _{n=0}^\infty (-1)^n\frac{(x/2)^{2n+1}}{(2n+1)}.</m>
        </p>
      </answer>
    </exercise>
    <exercise>
      <statement>
        <p>
          <m>f(x) = e^x\sin x</m> (only find the first 4 terms)</p>
      </statement>
      <answer>
        <p>
          <m>\displaystyle x+x^2+\frac{x^3}{3}-\frac{x^5}{30}</m>
        </p>
      </answer>
    </exercise>
    <exercise>
      <statement>
        <p>
          <m>f(x) = (1+x)^{1/2}\cos x</m> (only find the first 4 terms)</p>
      </statement>
      <answer>
        <p>
          <m>\displaystyle 1+\frac{x}{2}-\frac{5x^2}{8}-\frac{3x^3}{16}</m>
        </p>
      </answer>
    </exercise>
  </exercisegroup>
  <exercisegroup>
    <introduction>
      <p>
        In Exercises 31–32, approximate the value of the given definite integral by using the first 4 nonzero terms of the integrand's Taylor series.
        </p>
    </introduction>
    <exercise>
      <statement>
        <p>
          <m>\displaystyle \int _0^{\sqrt{\pi }} \sin \big (x^2\big )\ dx</m>
        </p>
      </statement>
      <answer>
        <p>
          <m>\displaystyle \int _0^{\sqrt{\pi }} \sin \big (x^2\big )\ dx \approx \int _0^{\sqrt{\pi }} \left(x^2-\frac{x^6}{6}+\frac{x^{10}}{120}-\frac{x^{14}}{5040}\right) dx = 0.8877</m>
        </p>
      </answer>
    </exercise>
    <exercise>
      <statement>
        <p>
          <m>\displaystyle \int _0^{\pi ^2/4} \cos \big (\sqrt{x}\big )\ dx</m>
        </p>
      </statement>
      <answer>
        <p>
          <m>\displaystyle \int _0^{\pi ^2/4} \cos \big (\sqrt{x}\big )\ dx \approx \int _0^{\pi ^2/4} \left(1-\frac{x}{2}+\frac{x^2}{24}-\frac{x^3}{720}\right)\ dx = 1.1412</m>. (Actual answer: <m>\pi -2</m>)</p>
      </answer>
    </exercise>
  </exercisegroup>
</exercises>
