<?xml version="1.0" encoding="UTF-8"?>
<exercises>
  <exercise>
    <statement>
      <p>
        What is the difference between a constant and a coefficient?
        </p>
    </statement>
    <answer>
      <p>
        A constant is a number that is added or subtracted in an expression; a coefficient is a number that is being multiplied by a nonconstant function.
        </p>
    </answer>
  </exercise>
  <exercise>
    <statement>
      <p>
        Given a function <m>z=f(x,y)</m>, explain in your own words how to compute <m>f_x</m>.
      </p>
    </statement>
    <answer>
      <p>
        Answers will vary; each should include something about treating <m>y</m> as a constant or a coefficient.
      </p>
    </answer>
  </exercise>
  <exercise>
    <statement>
      <p>
        In the mixed partial fraction <m>f_{xy}</m>, which is computed first, <m>f_x</m> or <m>f_y</m>?
      </p>
    </statement>
    <answer>
      <p>
        <m>f_x</m>
      </p>
    </answer>
  </exercise>
  <exercise>
    <statement>
      <p>
        In the mixed partial fraction <m>\displaystyle \frac{\partial ^2f}{\partial x\partial y}</m>, which is computed first, <m>f_x</m> or <m>f_y</m>?
      </p>
    </statement>
    <answer>
      <p>
        <m>f_y</m>
      </p>
    </answer>
  </exercise>
  <exercisegroup>
    <introduction>
      <p>
        Evaluate <m>f_x(x,y)</m> and <m>f_y(x,y)</m> at the indicated point.
      </p>
    </introduction>
    <exercise>
      <statement>
        <p>
          <m>f(x,y) = x^2y-x+2y+3</m> at <m>(1,2)</m>
        </p>
      </statement>
      <answer>
        <p>
          <m>f_x=2xy-1</m>, <m>f_y=x^2+2</m>
          <m>f_x(1,2) = 3</m>, <m>f_y(1,2) = 3</m>
        </p>
      </answer>
    </exercise>
    <exercise>
      <statement>
        <p>
          <m>f(x,y) = x^3-3x+y^2-6y</m> at <m>(-1,3)</m>
        </p>
      </statement>
      <answer>
        <p>
          <m>f_x=3x^2-3</m>, <m>f_y=2y-6</m>
          <m>f_x(-1,3) = 0</m>, <m>f_y(-1,3) = 0</m>
        </p>
      </answer>
    </exercise>
    <exercise>
      <statement>
        <p>
          <m>f(x,y) = \sin y\cos x</m> at <m>(\pi /3,\pi /3)</m>
        </p>
      </statement>
      <answer>
        <p>
          <m>f_x=-\sin x\sin y</m>, <m>f_y=\cos x\cos y</m>
          <m>f_x(\pi /3,\pi /3) = -3/4</m>, <m>f_y(\pi /3,\pi /3) = 1/4</m>
        </p>
      </answer>
    </exercise>
    <exercise>
      <statement>
        <p>
          <m>f(x,y) = \ln (xy)</m> at <m>(-2,-3)</m>
        </p>
      </statement>
      <answer>
        <p>
          <m>f_x=1/x</m>, <m>f_y=1/y</m>
          <m>f_x(-2,-3) = -1/2</m>, <m>f_y(-2,-3) = -1/3</m>
        </p>
      </answer>
    </exercise>
  </exercisegroup>
  <exercisegroup>
    <introduction>
      <p>
        Find <m>f_x</m>,  <m>f_y</m>,  <m>f_{xx}</m>,  <m>f_{yy}</m>,  <m>f_{xy}</m> and <m>f_{yx}</m>.
      </p>
    </introduction>
    <exercise>
      <statement>
        <p>
          <m>f(x,y) = x^2y+3x^2+4y-5</m>
        </p>
      </statement>
      <answer>
        <p>
          <m>f_x=2xy+6x</m>, <m>f_y=x^2+4</m>
          <m>f_{xx}=2y+6</m>, <m>f_{yy}=0</m>
          <m>f_{xy}=2x</m>, <m>f_{yx}=2x</m>
        </p>
      </answer>
    </exercise>
    <exercise>
      <statement>
        <p>
          <m>f(x,y) = y^3+3xy^2+3x^2y+x^3</m>
        </p>
      </statement>
      <answer>
        <p>
          <m>f_x=3x^2+6xy+3y^2</m>, <m>f_y=3x^2+6xy+3y^2</m>
          <m>f_{xx}=6x+6y</m>, <m>f_{yy}=6x+6y</m>
          <m>f_{xy}=6x+6y</m>, <m>f_{yx}=6x+6y</m>
        </p>
      </answer>
    </exercise>
    <exercise>
      <statement>
        <p>
          <m>\displaystyle f(x,y) = \frac{x}{y}</m>
        </p>
      </statement>
      <answer>
        <p>
          <m>f_x=1/y</m>, <m>f_y=-x/y^2</m>
          <m>f_{xx}=0</m>, <m>f_{yy}=2x/y^3</m>
          <m>f_{xy}=-1/y^2</m>, <m>f_{yx}=-1/y^2</m>
        </p>
      </answer>
    </exercise>
    <exercise>
      <statement>
        <p>
          <m>\displaystyle f(x,y) = \frac{4}{xy}</m>
        </p>
      </statement>
      <answer>
        <p>
          <m>f_x=-4/(x^2y)</m>, <m>f_y=-4/(xy^2)</m>
          <m>f_{xx}=8/(x^3y)</m>, <m>f_{yy}=8/(xy^3)</m>
          <m>f_{xy}=4/(x^2y^2)</m>, <m>f_{yx}=4/(x^2y^2)</m>
        </p>
      </answer>
    </exercise>
    <exercise>
      <statement>
        <p>
          <m>\displaystyle f(x,y) = e^{x^2+y^2}</m>
        </p>
      </statement>
      <answer>
        <p>
          <m>f_x=2xe^{x^2+y^2}</m>, <m>f_y=2ye^{x^2+y^2}</m>
          <m>f_{xx}=2e^{x^2+y^2}+4x^2e^{x^2+y^2}</m>, <m>f_{yy}=2e^{x^2+y^2}+4y^2e^{x^2+y^2}</m>
          <m>f_{xy}=4xye^{x^2+y^2}</m>, <m>f_{yx}=4xye^{x^2+y^2}</m>
        </p>
      </answer>
    </exercise>
    <exercise>
      <statement>
        <p>
          <m>\displaystyle f(x,y) = e^{x+2y}</m>
        </p>
      </statement>
      <answer>
        <p>
          <m>f_x=e^{x+2y}</m>, <m>f_y=2e^{x+2y}</m>
          <m>f_{xx}=e^{x+2y}</m>, <m>f_{yy}=4e^{x+2y}</m>
          <m>f_{xy}=2e^{x+2y}</m>, <m>f_{yx}=2e^{x+2y}</m>
        </p>
      </answer>
    </exercise>
    <exercise>
      <statement>
        <p>
          <m>\displaystyle f(x,y) = \sin x\cos y</m>
        </p>
      </statement>
      <answer>
        <p>
          <m>f_x=\cos x\cos y</m>, <m>f_y=-\sin x\sin y</m>
          <m>f_{xx}=-\sin x\cos y</m>, <m>f_{yy}=-\sin x\cos y</m>
          <m>f_{xy}=-\sin y\cos x</m>, <m>f_{yx}=-\sin y\cos x</m>
        </p>
      </answer>
    </exercise>
    <exercise>
      <statement>
        <p>
          <m>\displaystyle f(x,y) = (x+y)^3</m>
        </p>
      </statement>
      <answer>
        <p>
          <m>f_x=3(x+y)^2</m>, <m>f_y=3(x+y)^2</m>
          <m>f_{xx}=6(x+y)</m>, <m>f_{yy}=6(x+y)</m>
          <m>f_{xy}=6(x+y)</m>, <m>f_{yx}=6(x+y)</m>
        </p>
      </answer>
    </exercise>
    <exercise>
      <statement>
        <p>
          <m>f(x,y) = \cos (5xy^3)</m>
        </p>
      </statement>
      <answer>
        <p>
          <m>f_x=-5y^3\sin (5xy^3)</m>, <m>f_y=-15xy^2\sin (5xy^3)</m>
          <m>f_{xx}=-25y^6\cos (5xy^3)</m>, <m>f_{yy}=-225x^2y^4\cos (5xy^3)-30xy\sin (5xy^3)</m>
          <m>f_{xy}=-75xy^5\cos (5xy^3)-15y^2\sin (5xy^3)</m>, <m>f_{yx}=-75xy^5\cos (5xy^3)-15y^2\sin (5xy^3)</m>
        </p>
      </answer>
    </exercise>
    <exercise>
      <statement>
        <p>
          <m>f(x,y) = \sin (5x^2+2y^3)</m>
        </p>
      </statement>
      <answer>
        <p>
          <m>f_x=10x\cos (5x^2+2y^3)</m>, <m>f_y=6y^2\cos (5x^2+2y^3)</m>
          <m>f_{xx}=10\cos (5x^2+2y^3)-100x^2\sin (5x^2+2y^3)</m>, <m>f_{yy}=12y\cos (5x^2+2y^3)-36y^4\sin (5x^2+2y^3)</m>
          <m>f_{xy}=-60xy^2\sin (5x^2+2y^3)</m>, <m>f_{yx}=-60xy^2\sin (5x^2+2y^3)</m>
        </p>
      </answer>
    </exercise>
    <exercise>
      <statement>
        <p>
          <m>\displaystyle f(x,y) = \sqrt{4xy^2+1}</m>
        </p>
      </statement>
      <answer>
        <p>
          <m>f_x=\frac{2y^2}{\sqrt{4xy^2+1}}</m>, <m>f_y=\frac{4xy}{\sqrt{4xy^2+1}}</m>
          <m>f_{xx}=-\frac{4y^4}{\sqrt{4xy^2+1}^3}</m>, <m>f_{yy}=-\frac{16x^2y^2}{\sqrt{4xy^2+1}^3}+\frac{4x}{\sqrt{4xy^2+1}}</m>
          <m>f_{xy}=-\frac{8xy^3}{\sqrt{4xy^2+1}^3}+\frac{4y}{\sqrt{4xy^2+1}}</m>, <m>f_{yx}=-\frac{8xy^3}{\sqrt{4xy^2+1}^3}+\frac{4y}{\sqrt{4xy^2+1}}</m>
        </p>
      </answer>
    </exercise>
    <exercise>
      <statement>
        <p>
          <m>\displaystyle f(x,y) =(2x+5y)\sqrt{y}</m>
        </p>
      </statement>
      <answer>
        <p>
          <m>f_x=2\sqrt{y}</m>, <m>f_y=5\sqrt{y}+\frac{2x+5y}{2\sqrt{y}}</m>
          <m>f_{xx}=0</m>, <m>f_{yy}=\frac{5}{\sqrt{y}}-\frac{2x+5y}{4y^{3/2}}</m>
          <m>f_{xy}=\frac{1}{\sqrt{y}}</m>, <m>f_{yx}=\frac{1}{\sqrt{y}}</m>
        </p>
      </answer>
    </exercise>
    <exercise>
      <statement>
        <p>
          <m>\displaystyle f(x,y) =\frac{1}{x^2+y^2+1}</m>
        </p>
      </statement>
      <answer>
        <p>
          <m>f_x=-\frac{2x}{(x^2+y^2+1)^2}</m>, <m>f_y=-\frac{2y}{(x^2+y^2+1)^2}</m>
          <m>f_{xx}=\frac{8x^2}{(x^2+y^2+1)^3}-\frac{2}{(x^2+y^2+1)^2}</m>, <m>f_{yy}=\frac{8y^2}{(x^2+y^2+1)^3}-\frac{2}{(x^2+y^2+1)^2}</m>
          <m>f_{xy}=\frac{8xy}{(x^2+y^2+1)^3}</m>, <m>f_{yx}=\frac{8xy}{(x^2+y^2+1)^3}</m>
        </p>
      </answer>
    </exercise>
    <exercise>
      <statement>
        <p>
          <m>\displaystyle f(x,y) =5x-17y</m>
        </p>
      </statement>
      <answer>
        <p>
          <m>f_x=5</m>, <m>f_y=-17</m>
          <m>f_{xx}=0</m>, <m>f_{yy}=0</m>
          <m>f_{xy}=0</m>, <m>f_{yx}=0</m>
        </p>
      </answer>
    </exercise>
    <exercise>
      <statement>
        <p>
          <m>\displaystyle f(x,y) =3x^2+1</m>
        </p>
      </statement>
      <answer>
        <p>
          <m>f_x=6x</m>, <m>f_y=0</m>
          <m>f_{xx}=6</m>, <m>f_{yy}=0</m>
          <m>f_{xy}=0</m>, <m>f_{yx}=0</m>
        </p>
      </answer>
    </exercise>
    <exercise>
      <statement>
        <p>
          <m>\displaystyle f(x,y) =\ln (x^2+y)</m>
        </p>
      </statement>
      <answer>
        <p>
          <m>f_x=\frac{2x}{(x^2+y)}</m>, <m>f_y=\frac{1}{(x^2+y)}</m>
          <m>f_{xx}=-\frac{4x^2}{(x^2+y)^2}+\frac{2}{(x^2+y)}</m>, <m>f_{yy}=-\frac{1}{(x^2+y)^2}</m>
          <m>f_{xy}=-\frac{2x}{(x^2+y)^2}</m>, <m>f_{yx}=-\frac{2x}{(x^2+y)^2}</m>
        </p>
      </answer>
    </exercise>
    <exercise>
      <statement>
        <p>
          <m>\displaystyle f(x,y) =\frac{\ln x}{4y}</m>
        </p>
      </statement>
      <answer>
        <p>
          <m>f_x=\frac{1}{4xy}</m>, <m>f_y=-\frac{\ln x}{4y^2}</m>
          <m>f_{xx}=-\frac{1}{4x^2y}</m>, <m>f_{yy}=\frac{\ln x}{2y^3}</m>
          <m>f_{xy}=-\frac{1}{4xy^2}</m>, <m>f_{yx}=-\frac{1}{4xy^2}</m>
        </p>
      </answer>
    </exercise>
    <exercise>
      <statement>
        <p>
          <m>\displaystyle f(x,y) =5e^x\sin y+9</m>
        </p>
      </statement>
      <answer>
        <p>
          <m>f_x=5e^x\sin y</m>, <m>f_y=5e^x\cos y</m>
          <m>f_{xx}=5e^x\sin y</m>, <m>f_{yy}=-5e^x\sin y</m>
          <m>f_{xy}=5e^x\cos y</m>, <m>f_{yx}=5e^x\cos y</m>
        </p>
      </answer>
    </exercise>
  </exercisegroup>
  <exercisegroup>
    <introduction>
      <p>
        Form a function <m>z=f(x,y)</m> such that <m>f_x</m> and <m>f_y</m> match those given.
      </p>
    </introduction>
    <exercise>
      <statement>
        <p>
          <m>f_x = \sin y+1</m>,   <m>f_y = x\cos y</m>
        </p>
      </statement>
      <answer>
        <p>
          <m>f(x,y) = x\sin y+ x+ C</m>, where <m>C</m> is any constant.</p>
      </answer>
    </exercise>
    <exercise>
      <statement>
        <p>
          <m>f_x = x+y</m>,   <m>f_y = x+ y</m>
        </p>
      </statement>
      <answer>
        <p>
          <m>f(x,y) = \frac{1}{2}x^2+xy+\frac{1}{2}y^2+ C</m>, where <m>C</m> is any constant.</p>
      </answer>
    </exercise>
    <exercise>
      <statement>
        <p>
          <m>f_x = 6xy-4y^2</m>,   <m>f_y = 3x^2-8xy+2</m>
        </p>
      </statement>
      <answer>
        <p>
          <m>f(x,y) = 3x^2y-4xy^2+2y +C</m>, where <m>C</m> is any constant.</p>
      </answer>
    </exercise>
    <exercise>
      <statement>
        <p>
          <m>\displaystyle f_x = \frac{2x}{x^2+y^2}</m>,   <m>\displaystyle f_y = \frac{2y}{x^2+y^2}</m>
        </p>
      </statement>
      <answer>
        <p>
          <m>f(x,y) = \ln (x^2+y^2)+ C</m>, where <m>C</m> is any constant.</p>
      </answer>
    </exercise>
  </exercisegroup>
  <exercisegroup>
    <introduction>
      <p>
        Find <m>f_x</m>,  <m>f_y</m>,  <m>f_z</m>,  <m>f_{yz}</m> and <m>f_{zy}</m>.
      </p>
    </introduction>
    <exercise>
      <statement>
        <p>
          <m>\displaystyle f(x,y,z) = x^2e^{2y-3z}</m>
        </p>
      </statement>
      <answer>
        <p>
          <m>f_x = 2xe^{2y-3z}</m>, <m>f_y = 2x^2e^{2y-3z}</m>, <m>f_z = -3x^2e^{2y-3z}</m>
          <m>f_{yz} = -6x^2e^{2y-3z}</m>, <m>f_{zy} = -6x^2e^{2y-3z}</m>
        </p>
      </answer>
    </exercise>
    <exercise>
      <statement>
        <p>
          <m>\displaystyle f(x,y,z) = x^3y^2+x^3z+y^2z</m>
        </p>
      </statement>
      <answer>
        <p>
          <m>f_x = 3x^2y^2+3x^2z</m>, <m>f_y = 2x^3y+2yz</m>, <m>f_z = x^3+y^2</m>
          <m>f_{yz} = 2y</m>, <m>f_{zy} = 2y</m>
        </p>
      </answer>
    </exercise>
    <exercise>
      <statement>
        <p>
          <m>\displaystyle f(x,y,z) = \frac{3x}{7y^2z}</m>
        </p>
      </statement>
      <answer>
        <p>
          <m>f_x = \frac{3}{7y^2z}</m>, <m>f_y = -\frac{6x}{7y^3z}</m>, <m>f_z = -\frac{3x}{7y^2z^2}</m>
          <m>f_{yz} = \frac{6x}{7y^3z^2}</m>, <m>f_{zy} = \frac{6x}{7y^3z^2}</m>
        </p>
      </answer>
    </exercise>
    <exercise>
      <statement>
        <p>
          <m>\displaystyle f(x,y,z) = \ln (xyz)</m>
        </p>
      </statement>
      <answer>
        <p>
          <m>f_x = \frac{1}{x}</m>, <m>f_y = \frac{1}{y}</m>, <m>f_z = \frac{1}{z}</m>
          <m>f_{yz} = 0</m>, <m>f_{zy} = 0</m>
        </p>
      </answer>
    </exercise>
  </exercisegroup>
</exercises>
