<?xml version="1.0" encoding="UTF-8"?>
<exercises>
  <exercisegroup>
    <introduction>
      <p>
        In Exercises 1–8, Find the general solution to the first order linear differential equation.
        </p>
    </introduction>
    <exercise>
      <statement>
        <p>
          <m>\displaystyle y'= 2y - 3</m>
        </p>
      </statement>
      <answer>
        <p>
          <m>y = \displaystyle \frac{3}{2} + Ce^{2x}</m>
        </p>
      </answer>
    </exercise>
    <exercise>
      <statement>
        <p>
          <m>\displaystyle x^2y'+ xy = 1</m>
        </p>
      </statement>
      <answer>
        <p>
          <m>y = \displaystyle \frac{\ln |x| + C}{x}</m>
        </p>
      </answer>
    </exercise>
    <exercise>
      <statement>
        <p>
          <m>\displaystyle x^2y'- xy = 1</m>
        </p>
      </statement>
      <answer>
        <p>
          <m>y = \displaystyle -\frac{1}{2x} + Cx</m>
        </p>
      </answer>
    </exercise>
    <exercise>
      <statement>
        <p>
          <m>\displaystyle xy'+4y = x^3-x</m>
        </p>
      </statement>
      <answer>
        <p>
          <m>y = \displaystyle \frac{x^3}{7} - \frac{x}{5} + \frac{C}{x^4}</m>
        </p>
      </answer>
    </exercise>
    <exercise>
      <statement>
        <p>
          <m>\displaystyle (\cos ^2 x \sin x)y'+ (\cos ^3 x)y = 1</m>
        </p>
      </statement>
      <answer>
        <p>
          <m>y = \sec x + C(\csc x)</m>
        </p>
      </answer>
    </exercise>
    <exercise>
      <statement>
        <p>
          <m>\displaystyle \frac{y'}{x} = 1-2y</m>
        </p>
      </statement>
      <answer>
        <p>
          <m>y = \displaystyle \frac{1}{2} + Ce^{-x^2}</m>
        </p>
      </answer>
    </exercise>
    <exercise>
      <statement>
        <p>
          <m>\displaystyle x^3y'-3x^3y=x^4e^{2x}</m>
        </p>
      </statement>
      <answer>
        <p>
          <m>y = \displaystyle Ce^{3x}-(x+1)e^{2x}</m>
        </p>
      </answer>
    </exercise>
    <exercise>
      <statement>
        <p>
          <m>\displaystyle y'+ y = 5\sin (2x)</m>
        </p>
      </statement>
      <answer>
        <p>
          <m>y = sin(2x) - 2\cos (2x) + Ce^{-x}</m>
        </p>
      </answer>
    </exercise>
  </exercisegroup>
  <exercisegroup>
    <introduction>
      <p>
        In Exercises 9–16, Find the particular solution to the initial value problem.
        </p>
    </introduction>
    <exercise>
      <statement>
        <p>
          <m>\displaystyle y'= y + 2xe^x</m>,      <m>y(0) = 2</m>
        </p>
      </statement>
      <answer>
        <p>
          <m>y = (x^2+2)e^x</m>
        </p>
      </answer>
    </exercise>
    <exercise>
      <statement>
        <p>
          <m>\displaystyle xy'+ 2y = x^2 - x + 1</m>,      <m>y(1) = 1</m>
        </p>
      </statement>
      <answer>
        <p>
          <m>y = \displaystyle \frac{1}{4}x^2-\frac{1}{3}x+\frac{1}{2}+\frac{7}{12x^2}</m>
        </p>
      </answer>
    </exercise>
    <exercise>
      <statement>
        <p>
          <m>\displaystyle xy'+ (x+2)y = x</m>,      <m>y(1) = 0</m>
        </p>
      </statement>
      <answer>
        <p>
          <m>y = \displaystyle 1 - \frac{2}{x} + \frac{2-e^{1-x}}{x^2}</m>
        </p>
      </answer>
    </exercise>
    <exercise>
      <statement>
        <p>
          <m>\displaystyle y'+ 2y = 0</m>,      <m>y(0) = 3</m>
        </p>
      </statement>
      <answer>
        <p>
          <m>y = \displaystyle 3e^{-2x}</m>
        </p>
      </answer>
    </exercise>
    <exercise>
      <statement>
        <p>
          <m>\displaystyle (x+1)y'+ (x+2)y = 2xe^{-x}</m>,      <m>y(0) = 1</m>
        </p>
      </statement>
      <answer>
        <p>
          <m>y = \displaystyle \frac{x^2+1}{x+1}e^{-x}</m>
        </p>
      </answer>
    </exercise>
    <exercise>
      <statement>
        <p>
          <m>\displaystyle (\cos x)y'+ (\sin x)y = 1</m>,      <m>y(0) = -3</m>
        </p>
      </statement>
      <answer>
        <p>
          <m>y = \sin x - 3\cos x</m>
        </p>
      </answer>
    </exercise>
    <exercise>
      <statement>
        <p>
          <m>\displaystyle (x^2-1)y'+ 2y = (x+1)^2</m>,      <m>y(0) = 2</m>
        </p>
      </statement>
      <answer>
        <p>
          <m>y = \displaystyle \frac{(x-2)(x+1)}{x-1}</m>
        </p>
      </answer>
    </exercise>
    <exercise>
      <statement>
        <p>
          <m>\displaystyle xy'-2y = \frac{x^3}{1+x^2}</m>,      <m>y(1) = 0</m>
        </p>
      </statement>
      <answer>
        <p>
          <m>y = \displaystyle x^2\left(\arctan x - \frac{\pi }{4}\right)</m>
        </p>
      </answer>
    </exercise>
  </exercisegroup>
  <exercisegroup>
    <introduction>
      <p>
        In Exercises 17–20, classify the differential equation as separable, first order linear, or both, and solve the initial value problem using an appropriate method.
        </p>
    </introduction>
    <exercise>
      <statement>
        <p>
          <m>\displaystyle y'= y + yx^2</m>,      <m>y(0) = -5</m>
        </p>
      </statement>
      <answer>
        <p>
          Both; <m>\displaystyle y = -5e^{x + \frac{1}{3}x^3}</m>
        </p>
      </answer>
    </exercise>
    <exercise>
      <statement>
        <p>
          <m>\displaystyle xe^y y'= x^2\sin x</m>,      <m>y(0) = 0</m>
        </p>
      </statement>
      <answer>
        <p>
          separable; <m>\displaystyle e^y = \sin x - x\cos x + 1</m>
        </p>
      </answer>
    </exercise>
    <exercise>
      <statement>
        <p>
          <m>\displaystyle (x-1)y'+y = x^2-1</m>,      <m>y(0) = 2</m>
        </p>
      </statement>
      <answer>
        <p>
          linear; <m>\displaystyle y = \frac{x^3-3x-6}{3(x-1)}</m>
        </p>
      </answer>
    </exercise>
    <exercise>
      <statement>
        <p>
          <m>\displaystyle y'= y^2+y-2</m>,      <m>y(0) = 1</m>
        </p>
      </statement>
      <answer>
        <p>
          separable; <m>\displaystyle y = 1</m>
        </p>
      </answer>
    </exercise>
  </exercisegroup>
  <exercisegroup>
    <introduction>
      <p>
        In Exercises 21–22, draw a slope field for the differential equation. Use the slope field to predict the behavior of the solution to the initial value problem for large <m>x</m> values. Solve the initial value problem, and verify your prediction.
      </p>
    </introduction>
    <exercise>
      <statement>
        <p>
          <m>\displaystyle y'= x-y</m>,      <m>y(0) = 0</m>
        </p>
      </statement>
      <answer>
        <p>
          <m>y=x-1</m>, <m>y = x-1 + e^{-x}</m>
          <sidebyside width="30%">
            <image xml:id="img_diffeq_linear_ex1">
              <latex-image>
                \def\length{sqrt(1+(x - y)^2)}
                \begin{tikzpicture}
                \begin{axis}[width=\marginparwidth+25pt,
                tick label style={font=\scriptsize},
                axis lines = center,
                name=myplot,%
                view={0}{90},
                y domain = -.15:4,
                domain = -.15:4,
                ]
                \addplot3 [{\colortwo},quiver = {u = {1/(\length)}, v = {(x-y)/(\length)},scale arrows=.2},samples=15]{0};
                \addplot [{\colorone},thick,domain=0:4.1,samples=50] {x-1+exp(-x)};
                \end{axis}
                \node [right] at (myplot.right of origin) {\scriptsize $x$};
                \node [above] at (myplot.above origin) {\scriptsize $y$};
                \end{tikzpicture}
              </latex-image>
            </image>
          </sidebyside>
        </p>
      </answer>
    </exercise>
    <exercise>
      <statement>
        <p>
          <m>\displaystyle (x+1)y'+ y = \frac{1}{x+1}</m>,   <m>y(0) = 2</m>
        </p>
      </statement>
      <answer>
        <p>
          <m>y=0</m>, <m>\displaystyle y = \frac{2 + \ln (x+1)}{x+1}</m>
          <sidebyside width="30%">
            <image xml:id="img_diffeq_linear_ex2">
              <latex-image>
                \def\length{sqrt(1+(-y/(x+1)+1/(x+1)^2)^2)}
                \begin{tikzpicture}
                \begin{axis}[width=\marginparwidth+25pt,
                tick label style={font=\scriptsize},
                %axis y line=middle,axis x line=middle,
                axis lines = center,
                name=myplot,%
                view={0}{90},
                y domain = -.15:3,
                domain = -.15:4,
                ]
                \addplot3 [{\colortwo},quiver = {u = {1/(\length)}, v = {(-y/(x+1)+1/(x+1)^2)/(\length)},scale arrows=.2},samples=15]{0};
                \addplot [{\colorone},thick,domain=0:4.15,samples=50] {(2+ln(x+1))/(x+1)};
                \end{axis}
                \node [right] at (myplot.right of origin) {\scriptsize $x$};
                \node [above] at (myplot.above origin) {\scriptsize $y$};
                \end{tikzpicture}
              </latex-image>
            </image>
          </sidebyside>
        </p>
      </answer>
    </exercise>
  </exercisegroup>
</exercises>
