<?xml version="1.0" encoding="UTF-8"?>
<section xmlns:xi="http://www.w3.org/2001/XInclude" xml:id="sec_deriv_inverse_function">
  <title>Derivatives of Inverse Functions</title>
  <p>
    Recall that a function <m>y=f(x)</m> is said to be <term>one-to-one</term> if it passes the horizontal line test; that is, for two different <m>x</m>-values <m>x_1</m> and <m>x_2</m>, we do <em>not</em> have <m>f\mathopen{}\left(x_1\right)\mathclose{}=f\mathopen{}\left(x_2\right)\mathclose{}</m>. In some cases the domain of <m>f</m> must be restricted so that it is one-to-one. For instance, consider <m>f(x)=x^2</m>. Clearly, <m>f(-1)= f(1)</m>, so <m>f</m> is not one-to-one on its regular domain, but by restricting <m>f</m> to <m>(0,\infty)</m>, <m>f</m> is one-to-one.<idx><h>derivative</h>inverse function</idx>
  </p>
  <p>
    Now recall that one-to-one functions have <term>inverses</term>. That is, if <m>f</m> is one-to-one, it has an inverse function, denoted by <m>f^{-1}</m>, such that if <m>f(a)=b</m>, then <m>f^{-1}(b) = a</m>. The domain of <m>f^{-1}</m> is the range of <m>f</m>, and vice-versa. For ease of notation, we set <m>g=f^{-1}</m> and treat <m>g</m> as a function of <m>x</m>.
  </p>
  <p>
    Since <m>f(a)=b</m> implies <m>g(b)=a</m>, when we compose <m>f</m> and <m>g</m> we get a nice result:
      <me>
        f\big(g(b)\big) = f(a) = b.
      </me>
    
  </p>
  <p>
    In general, <m>f\big(g(x)\big) = x</m> and <m>g\big(f(x)\big) = x</m>. This gives us a convenient way to check if two functions are inverses of each other: compose them and if the result is <m>x</m> (on the appropriate domains), then they are inverses.
  </p>
  <p>
    When the point <m>(a,b)</m> lies on the graph of <m>f</m>, the point <m>(b,a)</m> lies on the graph of <m>g</m>. This leads us to discover that the graph of <m>g</m> is the reflection of <m>f</m> across the line <m>y=x</m>. In <xref ref="fig_inverse1">Figure</xref> we see a function graphed along with its inverse. See how the point <m>(1,1.5)</m> lies on one graph, whereas <m>(1.5,1)</m> lies on the other. Because of this relationship, whatever we know about <m>f</m> can quickly be transferred into knowledge about <m>g</m>.
  </p>
  <sidebyside width="47%">
    <figure xml:id="fig_inverse1">
      <caption>A function <m>f</m> along with its inverse <m>f^{-1}</m>. (Note how it does not matter which function we refer to as <m>f</m>; the other is <m>f^{-1}</m>.)</caption>
      <image xml:id="img_inverse1">
        <description />
        <latex-image>
            
            \begin{tikzpicture}
              \begin{axis}[axis equal image,
                           ymin=-1.3,ymax=2,
                           xmin=-1.3,xmax=2,
                           clip=false]
                \addplot+[domain=-1:1.14] ({x},{x^3+.5});
                \addplot+[domain=-1:1.14] ({x^3+.5},{x});
                \addplot [symmetryline] coordinates {(-1.3,-1.3) (1.7,1.7)};
                \addplot [soliddot] coordinates{(-.5,.375)} node[above left] {$(-0.5,0.375)$};
                \addplot [soliddot] coordinates{(.375,-.5)} node[below right] {$(0.375,-0.5)$};
                \addplot [soliddot] coordinates{(1,1.5)} node[above left] {$(1,1.5)$};
                \addplot [soliddot] coordinates{(1.5,1)} node[below right] {$(1.5,1)$};
              \end{axis}
            \end{tikzpicture}
            
          </latex-image>
      </image>
    </figure>
  </sidebyside>
  <p>
    For example, consider <xref ref="fig_inverse2">Figure</xref> where the tangent line to <m>f</m> at the point <m>(1,1.5)</m> is drawn. That line has slope <m>3</m>. Through reflection across <m>y=x</m>, we can see that the tangent line to <m>g</m> at the point <m>(1.5,1)</m> has slope <m>1/3</m>. Their slopes are reciprocals. This should make sense since reflecting a line (such as a tangent line) across the line <m>y=x</m> switches the <m>x</m> and <m>y</m> values. Also consider the point <m>(0,0.5)</m> on the graph of <m>f</m>, where the tangent line is horizontal. At the point <m>(0.5,0)</m> on <m>g</m>, the tangent line is vertical.
  </p>
  <p>
    More generally, consider the tangent line to <m>f</m> at the point <m>(a,b)</m>. That line has slope <m>\fp(a)</m>. Through reflection across <m>y=x</m>, we can extend our above observation to say that the tangent line to <m>g</m> at the point <m>(b,a)</m> should have slope <m>1/\fp(a)</m>. This then tells us that <m>g'(b)=1/\fp(a)</m>.
  </p>
  <sidebyside width="47%">
    <figure xml:id="fig_inverse2">
      <caption>Corresponding tangent lines drawn to <m>f</m> and <m>f^{-1}</m>.</caption>
      <image xml:id="img_inverse2">
        <description />
        <latex-image>
            
            \begin{tikzpicture}
              \begin{axis}[axis equal image,
                           ymin=-1.3,ymax=2,
                           xmin=-1.3,xmax=2,
                           clip=false,
                           grid=both,
                           xtick={-1,1},
                           ytick={-1,1},
                           minor xtick={-1.25,-1,...,2},
                           minor ytick={-1.25,-1,...,2},]
                \addplot+[domain=-1:1.14] ({x},{x^3+.5});
                \addplot+[domain=-1:1.14] ({x^3+.5},{x});
                \addplot [symmetryline] coordinates {(-1.3,-1.3) (1.7,1.7)};
                \addplot [tangentlineseg,domain=0.75:1.25]{3*(x-1)+1.5};
                \addplot [tangentlineseg,domain=0.75:2]{1/3*(x-1.5)+1};
                \addplot [soliddot] coordinates{(-.5,.375)} node[above left] {$(-0.5,0.375)$};
                \addplot [soliddot] coordinates{(.375,-.5)} node[below right] {$(0.375,-0.5)$};
                \addplot [soliddot] coordinates{(1,1.5)} node[above left] {$(1,1.5)$};
                \addplot [soliddot] coordinates{(1.5,1)} node[below right] {$(1.5,1)$};
              \end{axis}
            \end{tikzpicture}
            
          </latex-image>
      </image>
    </figure>
  </sidebyside>
  <p>
    The information from these two graphs is summarized in <xref ref="table_fandfinv"> Table </xref> below:
  </p>
  <table xml:id="table_fandfinv">
    <title />
    <tabular>
      <col halign="center" width="30%" />
      <col halign="center" width="30%" />
      <row bottom="medium">
        <cell>Information about <m>f</m>
        </cell>
        <cell>Information about <m>g=f^{-1}</m>
        </cell>
      </row>
      <row>
        <cell>
          <m>(1,1.5)</m> lies on <m>f</m>
        </cell>
        <cell>
          <m>(1.5,1)</m> lies on <m>g</m>
        </cell>
      </row>
      <row>
        <cell>
          <p>
            Slope of tangent line to <m>f</m> at <m>x=1</m> is <m>3</m>
          </p>
        </cell>
        <cell>
          <p>
            Slope of tangent line to <m>g</m> at <m>x=1.5</m> is <m>1/3</m>
          </p>
        </cell>
      </row>
      <row>
        <cell>
          <m>\fp(1) = 3</m>
        </cell>
        <cell>
          <m>g'(1.5) = 1/3</m>
        </cell>
      </row>
    </tabular>
  </table>
  <p>
    We have discovered a relationship between <m>\fp</m> and <m>g'</m> in a mostly graphical way. We can realize this relationship analytically as well. Let <m>y = g(x)</m>, where again <m>g = f^{-1}</m>. We want to find <m>y'</m>. Since <m>y = g(x)</m>, we know that <m>f(y) = x</m>. Using the <xref text="title" ref="thm_chain_rule" /> and Implicit Differentiation, take the derivative of both sides of this last equality.
      <md>
      <mrow>\lzoo{x}{f(y)} \amp = \lzoo{x}{x}</mrow>
      <mrow>\fp(y)\cdot y' \amp = 1</mrow>
      <mrow>y' \amp = \frac{1}{\fp(y)}</mrow>
      <mrow>y' \amp = \frac{1}{\fp(g(x))}</mrow>
    </md>
    
  </p>
  <p>
    This leads us to the following theorem.
    </p>
  <theorem xml:id="thm_deriv_inverse_functions">
    <title>Derivatives of Inverse Functions</title>
    <statement>
      <p>
        Let <m>f</m> be differentiable and one-to-one on an open interval <m>I</m>, where <m>\fp(x) \neq 0</m> for all <m>x</m> in <m>I</m>, let <m>J</m> be the range of <m>f</m> on <m>I</m>, let <m>g</m> be the inverse function of <m>f</m>, and let <m>f(a) = b</m> for some <m>a</m> in <m>I</m>. Then <m>g</m> is a differentiable function on <m>J</m>, and in particular,<ol cols="2">
          <li><m>\left(f^{-1}\right)'(b)=g'(b) = \dfrac{1}{\fp(a)}</m></li>
          <li><m>\left(f^{-1}\right)'(x)=g'(x) = \dfrac{1}{\fp(g(x))}</m></li>
        </ol>
      </p>
    </statement>
  </theorem>
  <p>
    The results of <xref ref="thm_deriv_inverse_functions">Theorem</xref> are not trivial; the notation may seem confusing at first. Careful consideration, along with examples, should earn understanding.
  </p>
  <p>
    In the next example we apply <xref ref="thm_deriv_inverse_functions">Theorem</xref> to the arcsine function.
  </p>
  <example xml:id="ex_deriv_arcsin">
    <title>Finding the derivative of an inverse trigonometric function</title>
    <statement>
      <p>
        Let <m>y = \arcsin(x) = \sin^{-1}(x)</m>. Find <m>y'</m> using <xref ref="thm_deriv_inverse_functions">Theorem</xref>.
      </p>
    </statement>
    <solution>
      <p>
        Adopting our previously defined notation, let <m>g(x) = \arcsin(x) </m> and <m>f(x) = \sin(x)</m>. Thus <m>\fp(x) = \cos(x)</m>. Applying the theorem, we have
          <md>
          <mrow>g'(x) \amp = \frac{1}{\fp(g(x))}</mrow>
          <mrow>\amp = \frac{1}{\cos(\arcsin(x))}.</mrow>
        </md>
        
      </p>
      <p>
        This last expression is not immediately illuminating. Drawing a figure will help, as shown in <xref ref="fig_inverse3">Figure</xref>. Recall that the sine function can be viewed as taking in an angle and returning a ratio of sides of a right triangle, specifically, the ratio <q>opposite over hypotenuse.</q> This means that the arcsine function takes as input a ratio of sides and returns an angle. The equation <m>y=\arcsin(x)</m> can be rewritten as <m>y=\arcsin(x/1)</m>; that is, consider a right triangle where the hypotenuse has length <m>1</m> and the side opposite of the angle with measure <m>y</m> has length <m>x</m>. This means the final side has length <m>\sqrt{1-x^2}</m>, using the Pythagorean Theorem.
      </p>
      <sidebyside width="47%">
        <figure xml:id="fig_inverse3">
          <caption>A right triangle defined by <m>y=\sin^{-1}(x/1)</m> with the length of the third leg found using the Pythagorean Theorem.</caption>
          <image xml:id="img_inverse3">
            <description />
            <latex-image>
                
                \begin{tikzpicture}
                  \coordinate (O) at (0,0);
                  \coordinate (A) at (5,0);
                  \coordinate (B) at (5,3.75);
                  \draw (O)--(A)--(B)--cycle;

                  \tkzLabelSegment[below=0pt](O,A){$\sqrt{1-x^2}$}
                  \tkzLabelSegment[above left=0pt](O,B){$1$}
                  \tkzLabelSegment[right=0pt](A,B){$x$}

                  \tkzMarkAngle[fill= orange,
                                size=1,
                                opacity=.4](A,O,B)
                  \tkzLabelAngle[pos = 0.75](A,O,B){$y$}
                \end{tikzpicture}
                
              </latex-image>
          </image>
        </figure>
      </sidebyside>
      <p>
        Therefore
          <md>
          <mrow>\cos\mathopen{}\left(\sin^{-1}(x)\right)\mathclose{} \amp= \cos(y)</mrow>
          <mrow>\amp = \frac{\sqrt{1-x^2}}{1}</mrow>
          <mrow>\amp = \sqrt{1-x^2},</mrow>
        </md>
        resulting in
          <me>
            \lzoo{x}{\arcsin(x)} = \frac{1}{\sqrt{1-x^2}}.
          </me>
        
      </p>
    </solution>
  </example>
  <p>
    Remember that the input <m>x</m> of the arcsine function is a ratio of a side of a right triangle to its hypotenuse; the absolute value of this ratio will never be greater than <m>1</m>. Therefore the inside of the square root will never be negative.
  </p>
  <p>
    In order to make <m>y=\sin(x)</m> one-to-one, we restrict its domain to <m>[-\pi/2,\pi/2]</m>; on this domain, the range is <m>[-1,1]</m>. Therefore the domain of <m>y=\arcsin(x)</m> is <m>[-1,1]</m> and the range is <m>[-\pi/2,\pi/2]</m>. When <m>x=\pm 1</m>, note how the derivative of the arcsine function is undefined; this corresponds to the fact that as <m>x\to \pm1</m>, the tangent lines to arcsine approach vertical lines with undefined slopes.
  </p>
  <figure xml:id="fig_inversesine">
    <caption>Graphs of <m>\sin(x)</m> and <m>\sin^{-1}(x)</m> along with corresponding tangent lines.</caption>
    <sidebyside widths="47% 47%">
        <image xml:id="img_inverse4">
          <description />
          <latex-image>
              
              \begin{tikzpicture}
                \begin{axis}[ymin=-1.7,ymax=1.7,
                             xmin=-1.7,xmax=1.7,
                             xtick={-1.57,-.79,.79,1.57},
                             xticklabels={$-\frac{\pi}{2}$,$-\frac{\pi}{4}$,$\frac{\pi}{4}$,$\frac{\pi}{2}$},
                             axis equal]

                  \addplot+[domain=-1.57:1.57,-] (x,{sin(deg(x))}) node [pos=0.5,above,sloped]{$y=\sin(x)$};
                  \addplot [tangentline,domain=.42:1.7] {.5*(x-pi/3)+sqrt(3)/2};
                  \addplot [soliddot] coordinates {(1.06,.866)} node [above left] {$\left(\frac{\pi}{3},\frac{\sqrt{3}}{2}\right)$};
              \end{axis}
              \end{tikzpicture}

              
            </latex-image>
        </image>
        <image xml:id="img_inverse5">
          <description />
          <latex-image>
              
              \begin{tikzpicture}
                \begin{axis}[ymin=-1.7,ymax=1.7,
                             xmin=-1.7,xmax=1.7,
                             ytick={-1.57,-.79,.79,1.57},
                             yticklabels={$-\frac{\pi}{2}$,$-\frac{\pi}{4}$,$\frac{\pi}{4}$,$\frac{\pi}{2}$},
                             axis equal]
                \addplot+[domain=-1.57:1.57,-] ({sin(deg(x))},x) node [pos=0.5,above,sloped]{$y=\sin^{-1}(x)$};
                \addplot [tangentline,domain=.42:1.7] ({.5*(x-pi/3)+sqrt(3)/2},{x});
                \addplot [soliddot] coordinates {(0.866,1.06)} node [below right] {$\left(\frac{\sqrt{3}}{2},\frac{\pi}{3}\right)$};
              \end{axis}
            \end{tikzpicture}
            
            </latex-image>
        </image>
    </sidebyside>
  </figure>
  <p>
    In <xref ref="fig_inversesine">Figure</xref> we see <m>f(x) = \sin(x)</m> and <m>f^{-1} = \sin^{-1}(x)</m> graphed on their respective domains. The line tangent to <m>\sin(x)</m> at the point <m>\left(\pi/3, \sqrt{3}/2\right)</m> has slope <m>\cos(\pi)/3 = 1/2</m>. The slope of the corresponding point on <m>\sin^{-1}(x)</m>, the point <m>\left(\sqrt{3}/2,\pi/3\right)</m>, is
      <md>
      <mrow>\frac{1}{\sqrt{1-\left(\sqrt{3}/2\right)^2}} \amp  = \frac{1}{\sqrt{1-3/4}}</mrow>
      <mrow> \amp = \frac{1}{\sqrt{1/4}}</mrow>
      <mrow> \amp = \frac{1}{1/2}=2</mrow>
    </md>
      verifying yet again that at corresponding points, a function and its inverse have reciprocal slopes.
  </p>
  <p>
    Using similar techniques, we can find the derivatives of all the inverse trigonometric functions. In <xref ref="table_domain_trig">Table</xref> we show the restrictions of the domains of the standard trigonometric functions that allow them to be invertible.
  </p>
  <table xml:id="table_domain_trig">
    <title>Domains and ranges of the trigonometric and inverse trigonometric functions.</title>
    <tabular>
      <row bottom="medium">
        <cell>Function</cell>
        <cell>Domain</cell>
        <cell>Range</cell>
      </row>
      <row>
        <cell>
          <m>\sin(x)</m>
        </cell>
        <cell>
          <m>[-\pi/2, \pi/2]</m>
        </cell>
        <cell>
          <m>[-1,1]</m>
        </cell>
      </row>
      <row>
        <cell>
          <m>\sin^{-1}(x)</m>
        </cell>
        <cell>
          <m>[-1,1]</m>
        </cell>
        <cell>
          <m>[-\pi/2, \pi/2]</m>
        </cell>
      </row>
      <row>
        <cell>
          <m>\cos(x)</m>
        </cell>
        <cell>
          <m>[0,\pi]</m>
        </cell>
        <cell>
          <m>[-1,1]</m>
        </cell>
      </row>
      <row>
        <cell>
          <m>\cos^{-1}(x)</m>
        </cell>
        <cell>
          <m>[-1,1]</m>
        </cell>
        <cell>
          <m>[0,\pi]</m>
        </cell>
      </row>
      <row>
        <cell>
          <m>\tan(x)</m>
        </cell>
        <cell>
          <m>(-\pi/2,\pi/2)</m>
        </cell>
        <cell>
          <m>(-\infty,\infty)</m>
        </cell>
      </row>
      <row>
        <cell>
          <m>\tan^{-1}(x)</m>
        </cell>
        <cell>
          <m>(-\infty,\infty)</m>
        </cell>
        <cell>
          <m>(-\pi/2,\pi/2)</m>
        </cell>
      </row>
      <row>
        <cell>
          <m>\csc(x)</m>
        </cell>
        <cell>
          <m>[-\pi/2,0)\cup (0, \pi/2]</m>
        </cell>
        <cell>
          <m>(-\infty,-1]\cup [1,\infty)</m>
        </cell>
      </row>
      <row>
        <cell>
          <m>\csc^{-1}(x)</m>
        </cell>
        <cell>
          <m>(-\infty,-1]\cup [1,\infty)</m>
        </cell>
        <cell>
          <m>[-\pi/2,0)\cup (0, \pi/2]</m>
        </cell>
      </row>
      <row>
        <cell>
          <m>\sec(x)</m>
        </cell>
        <cell>
          <m>[0,\pi/2)\cup (\pi/2,\pi]</m>
        </cell>
        <cell>
          <m>(-\infty,-1]\cup [1,\infty)</m>
        </cell>
      </row>
      <row>
        <cell>
          <m>\sec^{-1}(x)</m>
        </cell>
        <cell>
          <m>(-\infty,-1]\cup [1,\infty)</m>
        </cell>
        <cell>
          <m>[0,\pi/2)\cup (\pi/2,\pi]</m>
        </cell>
      </row>
      <row>
        <cell>
          <m>\cot(x)</m>
        </cell>
        <cell>
          <m>(0,\pi)</m>
        </cell>
        <cell>
          <m>(-\infty,\infty)</m>
        </cell>
      </row>
      <row>
        <cell>
          <m>\cot^{-1}(x)</m>
        </cell>
        <cell>
          <m>(-\infty,\infty)</m>
        </cell>
        <cell>
          <m>(0,\pi)</m>
        </cell>
      </row>
    </tabular>
  </table>
  <theorem xml:id="thm_deriv_inverse_trig">
    <title>Derivatives of Inverse Trigonometric Functions</title>
    <statement>
      <p>
        The inverse trigonometric functions are differentiable on all open sets contained in their domains (as listed in <xref ref="table_domain_trig">Table</xref>) and their derivatives are as follows:<ol>
          <li>
            <p><m>\displaystyle\lzoo{x}{\sin^{-1}(x)} = \frac{1}{\sqrt{1-x^2}}</m></p>
          </li>
          <li>
            <p><m>\displaystyle\lzoo{x}{\cos^{-1}(x)} = -\frac{1}{\sqrt{1-x^2}}</m></p>
          </li>
          <li>
            <p><m>\displaystyle\lzoo{x}{\tan^{-1}(x)} = \frac{1}{1+x^2}</m></p>
          </li>
          <li>
            <p><m>\displaystyle\lzoo{x}{\csc^{-1}(x)} = -\frac{1}{\abs{x}\sqrt{x^2-1}}</m></p>
          </li>
          <li>
            <p><m>\displaystyle\lzoo{x}{\sec^{-1}(x)} = \frac{1}{\abs{x}\sqrt{x^2-1}}</m></p>
          </li>
          <li>
            <p><m>\displaystyle\lzoo{x}{\cot^{-1}(x)} = -\frac{1}{1+x^2}</m></p>
          </li>
        </ol><idx><h>derivative</h>inverse trig.</idx>
      </p>
    </statement>
  </theorem>
  <p>
    Note how each derivative is the negative of the derivative of its <q>co</q> function. Because of this, derivatives of <m>\sin^{-1}(x)</m>, <m>\tan^{-1}(x)</m>, and <m>\sec^{-1}(x)</m> are used almost exclusively throughout this text.
  </p>
  <p>
    In <xref ref="sec_basic_diff_rules">Section</xref>, we stated without proof or explanation that <m>\lzoo{x}{\ln(x)}=\frac{1}{x}</m>. We can justify that now using <xref ref="thm_deriv_inverse_functions">Theorem</xref>, as shown in the example.
  </p>
  <example xml:id="ex_deriv_lnx">
    <title>Finding the derivative of <m>y=\ln(x)</m>
    </title>
    <statement>
      <p>
        Use <xref ref="thm_deriv_inverse_functions">Theorem</xref> to compute <m>\lzoo{x}{\ln(x)}</m>.
      </p>
    </statement>
    <solution>
      <p>
        View <m>y= \ln(x)</m> as the inverse of <m>y = e^x</m>. Therefore, using our standard notation, let <m>f(x) = e^x</m> and <m>g(x) = \ln(x)</m>. We wish to find <m>g'(x)</m>. <xref ref="thm_deriv_inverse_functions">Theorem</xref> gives:
          <md>
          <mrow>g'(x) \amp = \frac{1}{\fp(g(x))}</mrow>
          <mrow>\amp = \frac{1}{e^{\ln(x) }}</mrow>
          <mrow>\amp = \frac{1}{x}.</mrow>
        </md>
        
      </p>
    </solution>
  </example>
  <p>
    In this chapter we have defined the derivative, given rules to facilitate its computation, and given the derivatives of a number of standard functions. We restate the most important of these in the following theorem, intended to be a reference for further work.
    </p>
  <theorem xml:id="thm_deriv_glossary">
    <title>Glossary of Derivatives of Elementary Functions</title>
    <statement>
      <p>
        Let <m>f</m> and <m>g</m> be differentiable functions, and let <m>a</m>, <m>c</m> and <m>n</m> be real numbers, <m>a&gt;0</m>, <m>n\neq 0</m>.
      </p>
      <p>
        <ol cols="2">
          <li>
            <p>
              <m>\lzoo{x}{c\cdot f(x)} = c\cdot f'(x)</m>
            </p>
          </li>
          <li>
            <p>
              <m>\lzoo{x}{f(x)\pm g(x)} = f'(x) \pm g'(x)</m>
            </p>
          </li>
          <li>
            <p>
              <m>\lzoo{x}{f(x)\cdot g(x)} = f'(x)\cdot g(x)+f(x)\cdot g'(x)</m>
            </p>
          </li>
          <li>
            <p>
              <m>\lzoo{x}{\frac{f(x)}{g(x)}} = \frac{f'(x)\cdot g(x)-f(x) \cdot g'(x)}{(g(x))^2}</m>
            </p>
          </li>
          <li>
            <p>
              <m>\lzoo{x}{f(g(x))} = f'(g(x)) \cdot g'(x)</m>
            </p>
          </li>
          <li>
            <p>
              <m>\lzoo{x}{c} = 0</m>
            </p>
          </li>
          <li>
            <p>
              <m>\lzoo{x}{x} = 1</m>
            </p>
          </li>
          <li>
            <p>
              <m>\lzoo{x}{x^n} = nx^{n-1}</m>
            </p>
          </li>
          <li>
            <p>
              <m>\lzoo{x}{e^x} = e^x</m>
            </p>
          </li>
          <li>
            <p>
              <m>\lzoo{x}{\ln(x)} = \frac{1}{x}</m>
            </p>
          </li>
          <li>
            <p>
              <m>\lzoo{x}{a^x} = \ln(a)\cdot a^x</m>
            </p>
          </li>
          <li>
            <p>
              <m>\lzoo{x}{\log_a x} = \frac{1}{\ln(a)}\cdot\frac{1}{x}</m>
            </p>
          </li>
          <li>
            <p>
              <m>\lzoo{x}{\sin(x)} = \cos(x)</m>
            </p>
          </li>
          <li>
            <p>
              <m>\lzoo{x}{\cos(x)} = -\sin(x)</m>
            </p>
          </li>
          <li>
            <p>
              <m>\lzoo{x}{\tan(x)} = \sec^2(x)</m>
            </p>
          </li>
          <li>
            <p>
              <m>\lzoo{x}{\csc(x)} = -\csc(x)\cot(x)</m>
            </p>
          </li>
          <li>
            <p>
              <m>\lzoo{x}{\sec(x)} = \sec(x)\tan(x)</m>
            </p>
          </li>
          <li>
            <p>
              <m>\lzoo{x}{\cot(x)} = -\csc^2(x)</m>
            </p>
          </li>
          <li>
            <p>
              <m>\lzoo{x}{\sin^{-1}(x)} = \frac{1}{\sqrt{1-x^2}}</m>
            </p>
          </li>
          <li>
            <p>
              <m>\lzoo{x}{\cos^{-1}(x)} = -\frac{1}{\sqrt{1-x^2}}</m>
            </p>
          </li>
          <li>
            <p>
              <m>\lzoo{x}{\tan^{-1}(x)} = \frac{1}{1+x^2}</m>
            </p>
          </li>
          <li>
            <p>
              <m>\lzoo{x}{\csc^{-1}(x)} = -\frac{1}{\abs{x}\sqrt{x^2-1}}</m>
            </p>
          </li>
          <li>
            <p>
              <m>\lzoo{x}{\sec^{-1}(x)} = \frac{1}{\abs{x}\sqrt{x^2-1}}</m>
            </p>
          </li>
          <li>
            <p>
              <m>\lzoo{x}{\cot^{-1}(x)} = -\frac{1}{1+x^2}</m>
            </p>
          </li>
        </ol>
      </p>
    </statement>
  </theorem>
  <xi:include href="exer_sec_deriv_inverse_function.ptx" />
</section>
